<?xml version='1.0' encoding='utf-8'?>

<section xml:id="section-3536" xmlns:xi="http://www.w3.org/2001/XInclude">
	<title>Rate of Change of Product Functions</title>

	<subsection xml:id="section-3536-product">
		<title>Product Rule</title>
		
		<p>
			The <term>product rule</term> allows us to take derivatives of product functions, i.e. functions that look like <m>h(x) = f(x)\cdot g(x)</m>.  The product rule is
			<me>
				h'(x) = f'(x)g(x) + f(x)g'(x)
			</me>
			
		</p>

		<example>
			<statement>
				<p>
					Find the derivative of <m>h(x)</m>, where <m>h(x) = [4(3^x)]\cdot [5x^2]</m>
				</p>
			</statement>
			<solution>
				<p>
					<m>h'(x) = [4\ln3\cdot 3^x][5x^2] + [4(3^x)][10x]</m>
				</p>
			</solution>
		</example>

		<example>
			<statement>
				<p>
					Find the derivative of <m>g(y)=\dfrac{\ln (2y)}{1+y^2}</m>.  
				</p>
			</statement>
			<solution>
				<p>
					<m>g'(y) = \lrpar{\dfrac{1}{2y}\cdot 2}\lrpar{(1+y^2)^{-1}}+(\ln(2y))(-(1+y^2)^{-2}\cdot 2y)</m>
				</p>
			</solution>
		</example>

		<example>
			<statement>
				<p>
					Compute the derivative of the function <m>g(x) = 3x^{-0.7}\cdot 5^x</m> 
				</p>
			</statement>
			<solution>
				<p>
					<m>g'(x) = (-2.1x^{-1.7})(5^x)+(3x^{-0.7})(\ln 5\cdot 5^x)</m>
				</p>
			</solution>
		</example>

		<example>
			<statement>
				<p>
					Let <m>f(x) = 3\ln (2+5x)</m>, and <m>h(x) = \dfrac{1}{\ln x}</m>.  Find <m>(f\cdot h)'(x)</m>.
				</p>
			</statement>
			<solution>
				<p>
					<m>(f\cdot h)'(x) = \lrpar{\dfrac{3}{2+5x}\cdot 5}\lrpar{\dfrac{1}{\ln x}}+(3\ln(2+5x))\lrpar{-(\ln x)^{-2}\cdot \dfrac{1}{x}}</m>
				</p>
			</solution>
		</example>

		<example>
			<statement>
				<p>
					The profit from the supply of a certain commodity is modeled by <m>P(q) = 72qe^{-0.2q}</m> dollars, when <m>q</m> units are produced.
				</p>
				<p>
					<ol marker="a">
						<li>
							<p>
								Write the complete rate of change model for profit.
							</p>
						</li>
						<li>
							<p>
								At what production level(s) is the rate of change of profit zero?  If necessary, round your answer to two decimal places.  
							</p>
						</li>
						<li>
							<p>
								What is profit at the production level for the value in part (b)?  
							</p>
						</li>
					</ol>
				</p>
			</statement>
			<solution>
				<p>
					<ol marker="a">
						<li>
							<p>
								<m>P'(q) = 72e^{-0.2q} -14.4qe^{-0.2q}</m> dollars per unit, rate of change of profit from supply of a commodity, when <m>q</m> units are produced.
							</p>
						</li>
						<li>
							<p>
								<m>q = 5</m> units
							</p>
						</li>
						<li>
							<p>
								132.44 dollars 
							</p>
						</li>
					</ol>
				</p>
			</solution>
		</example>
	</subsection>

	<subsection xml:id="section-3536-quotient">
		<title>Quotient Rule</title>
		
		<p>
			Alternately, for a quotient function, we may employ the <term>quotient rule</term>.  If <m>k(x) = \dfrac{f(x)}{g(x)}</m>, then
			<me>
				k'(x) = \dfrac{f'(x)g(x) - f(x)g'(x)}{[g(x)]^2}
			</me>
			This can be remembered as
			<me>
				\dfrac{\text{low}\cdot d\text{(high)} - \text{high }\cdot d\text{(low)} }{\text{(low)}^2}
			</me>
		</p>

		<example>
			<statement>
				<p>
					Use the quotient rule to find the derivative of <m>g(y)=\dfrac{\ln (2y)}{1+y^2}</m> 
				</p>
			</statement>
			<solution>
				<p>
					<m>g'(y) = \dfrac{(1+y^2)\lrpar{\dfrac{1}{2y}\cdot 2}-(\ln(2y))(2y)}{(1+y^2)^2}</m>
				</p>
			</solution>
		</example>
	</subsection>

	<subsection xml:id="section-3536-examples">
		<title>Examples</title>
		
		<example>
			<statement>
				<p>
					The production level at a plant manufacturing radios can be modeled as <m>f(x) = 10.54x^{0.5}(2-0.13x)^{0.3}</m> thousand radios, where <m>x</m> thousand dollars has been spent on modernizing plant technology.
				</p>
				<p>
					<ol marker="a">
						<li>
							<p>
								Identify two functions <m>g</m> and <m>h</m> that, when multiplied, form the production model- one of the functions will need the chain rule
							</p>
						</li>
						<li>
							<p>
								Using function notation, write the notation for the production model and for the rate of change of the production model.  
							</p>
						</li>
						<li>
							<p>
								Write a model for the rate of change of production  
							</p>
						</li>
					</ol>
				</p>
			</statement>
			<solution>
				<p>
					<ol marker="a">
						<li>
							<p>
								Choose <m>g(x) = 10.54x^{0.5}</m> and <m>h(x) = (2-0.13x)^{0.3}</m>
							</p>
						</li>
						<li>
							<p>
								The production model is <m>f(x) = g(x)h(x) = (gh)(x)</m> and the rate of change model is <m>f'(x) = g'(x)h(x) + g(x)h'(x) = (gh)'(x)</m>
							</p>
						</li>
						<li>
							<p>
								<m>f'(x) = (5.27x^{-0.5})(2-0.13x)^{0.3} + (10.54x^{0.5})(0.3(2-0.13x)^{-0.7}\cdot -0.13)</m> thousand radios per thousand dollars, rate of change of production, where <m>x</m> thousand dollars has been spent on modernizing plant technology.
							</p>
						</li>
					</ol>
				</p>
			</solution>
		</example>

		<example>
			<statement>
				<p>
					Write the product function and rate-of-change function for the given functions.
				</p>
				<p>
					<ol marker="a">
						<li>
							<p>
								<m>g(x) = 5x^2 - 3</m> and <m>h(x) = 1.2^x</m>  
							</p>
						</li>
						<li>
							<p>
								<m>g(x) = 6e^{-x}+\ln x</m> and <m>h(x) = 4x^{2.1}</m> 
							</p>
						</li>
					</ol>
				</p>
			</statement>
			<solution>
				<p>
					<ol marker="a">
						<li>
							<p>
								<m>(gh)(x) = (5x^2-3)(1.2^x)</m>  and <m>(gh)'(x) = (10x)(1.2^x) + (5x^2-3)(\ln(1.2)\cdot 1.2^x)</m>
							</p>
						</li>
						<li>
							<p>
								<m>(gh)(x) = (6e^{-x}+\ln x)(4x^{2.1})</m> and <m>(gh)'(x) = \lrpar{-6e^{-x}+\dfrac{1}{x}}(4x^{2.1})+(6e^{-x}+\ln x)(8.2x^{1.1})</m>
							</p>
						</li>
					</ol>
				</p>
			</solution>
		</example>

		<example>
			<statement>
				<p>
					Find the derivatives of the following functions.
				</p>
				<p>
					<ol marker="a">
						<li>
							<p>
								<m>f(x) = (\ln x)e^x</m>
							</p>
						</li>
						<li>
							<p>
								<m>g(x) = (x+5)e^x</m>  
							</p>
						</li>
						<li>
							<p>
								<m>t(x) = (5.7x^2+3.5x+2.9)^3(3.8x^2+5.2x+7)^{-2}</m>
							</p>
						</li>
						<li>
							<p>
								<m>f(x) = \dfrac{2x^3+3}{2.7x+15}</m>
							</p>
						</li>
						<li>
							<p>
								<m>f(x) = (8x^2 + 13)\left(\dfrac{39}{1+15e^{-0.09x}}\right)</m>
							</p>
						</li>
						<li>
							<p>
								<m>f(x) = [\ln (15.7x^3)]\cdot [e^{15.7x^3}]</m> 
							</p>
						</li>
						<li>
							<p>
								<m>f(x) = \dfrac{4(3^x)}{\sqrt{x}}</m>
							</p>
						</li>
						<li>
							<p>
								<m>f(x) = \dfrac{14x}{1 + 12.6e^{-0.73x}}</m> 
							</p>
						</li>
					</ol>
				</p>
			</statement>
			<solution>
				<p>
					<ol marker="a">
						<li>
							<p>
								<m>f'(x) = \lrpar{\dfrac{1}{x}}(e^x} + (\ln x)(e^x)</m>
							</p>
						</li>
						<li>
							<p>
								<m>g'(x) = (1)(e^x) + (x+5)(e^x)</m>  
							</p>
						</li>
						<li>
							<p>
								<m>t'(x) = (3(5.7x^2+3.5x+2.9)^2(11.4x+3.5))((3.8x^2+5.2x+7)^{-2})+((5.7x^2+3.5x+2.9)^3)(-2(3.8x^2+5.2x+7)^{-3})(7.6x+5.2))</m>
							</p>
						</li>
						<li>
							<p>
								<m>f'(x) = \dfrac{(6x^2)(2.7x+15)-(2x^3+3)(2.7)}{(2.7x+15)^2}</m>
							</p>
						</li>
						<li>
							<p>
								<m>f'(x) = (16x)\lrpar{\dfrac{39}{1+15e^{-0.09x}}}+(8x^2+13)\lrpar{39(-1)(1+15e^{-0.09x})^{-2}\cdot (15e^{-0.09x}\cdot -0.09)}</m>
							</p>
						</li>
						<li>
							<p>
								<m>f'(x) = \lrpar{\dfrac{1}{15.7x^3}\cdot (15.7\cdot 3x^2)}(e^{15.7x^3}) + (\ln(15.7x^3))(15.7\cdot 3x^2\cdot e^{15.7x^3})</m> 
							</p>
						</li>
						<li>
							<p>
								<m>f'(x) = \dfrac{(4\ln 3\cdot 3^x)(\sqrt{x}) - (4(3^x))\lrpar{\dfrac{1}{2}x^{-1/2}}}{x}</m>
							</p>
						</li>
						<li>
							<p>
								<m>f'(x) = \dfrac{(14)({1 + 12.6e^{-0.73x})-(14x)(12.6e^{-0.73x}\cdot -0.73)}{(1 + 12.6e^{-0.73x})^2}</m> 
							</p>
						</li>
					</ol>
				</p>
			</solution>
		</example>

		<example>
			<statement>
				<p>
					A store has determined that the number of cookies sold monthly is approximately <m>c(x) = 6250(0.929^x)</m> cookies, where <m>x</m> is the average price of a cookie (in dollars).
				</p>
				<p>
					<ol marker="a">
						<li>
							<p>
								Write a model for revenue as a function of price.
							</p>
						</li>
						<li>
							<p>
								If each cookie costs the store $1, write a model for profit as a function of price.
							</p>
						</li>
						<li>
							<p>
								Write the complete rate of change model for revenue as a function of price.
							</p>
						</li>
					</ol>
				</p>
			</statement>
			<solution>
				<p>
					<ol marker="a">
						<li>
							<p>
								<m>R(x) = x\cdot c(x) = 6250x(0.929^x)</m> dollars, revenue from cookie sales, where <m>x</m> is the average price of a cookie (in dollars).
							</p>
						</li>
						<li>
							<p>
								<m>P(x) = R(x) - x = 6250x(0.929^x) -x</m> dollars, profit from cookie sales, where <m>x</m> is the average price of a cookie (in dollars).
							</p>
						</li>
						<li>
							<p>
								<m>R'(x) = 6250(0.929^x) + 6250\ln(0.929)x\cdot (0.929^x)</m> dollars revenue per dollar cookie price, rate of change of revenue from cookie sales, where <m>x</m> is the average price of a cookie (in dollars).
							</p>
						</li>
					</ol>
				</p>
			</solution>
		</example>

		<example>
			<statement>
				<p>
					Find the derivative of <m>t(x) = (6x^3)(\ln x)(e^{2x})</m>.
				</p>
			</statement>
			<solution>
				<p>
					<m>t'(x) = (18x^2)(\ln x)(e^{2x})+(6x^3)\lrpar{\dfrac{1}{x}}(e^{2x})+(6x^3)(\ln x)(2e^{2x})</m>
				</p>
			</solution>
		</example>
	</subsection>
</section>